ViewsProof.v
@@ -9,17 +9,17 @@ Require Import PeanoNat.
 (*
 preserve_Injectivity f <-> (fun (g : C -> ViewArray A) x y -> f (g x) y) preserves injectivity of g
 *)
-Definition preserve_Injectivity {l : nat} {A : List nat} {B : List nat} (f : ViewArray l A -> ViewArray l B) :=
-  forall (C : List nat) (v : ViewArray l (C++A)),
+Definition preserve_Injectivity {A : List nat} {B : List nat} (f : ViewArray A -> ViewArray B) :=
+  forall (C : List nat) (v : ViewArray (C++A)),
   Injective v ->
   (forall (i j : Tuple C) (x y : Tuple B),
   curry_totalApp (f (curry_partialApp v i)) x = curry_totalApp (f (curry_partialApp v j)) y -> (i,x) = (j,y)).
 
 Proposition preserve_Injectivity_implies_preserving_view_injectivity :
-  forall l A B (f : ViewArray l A -> ViewArray l B), preserve_Injectivity f -> (forall v, Injective v -> Injective (f v)).
+  forall A B (f : ViewArray A -> ViewArray B), preserve_Injectivity f -> (forall v, Injective v -> Injective (f v)).
 Proof.
   unfold preserve_Injectivity.
-  intros l A B f Hf v Hinj x y.
+  intros A B f Hf v Hinj x y.
   unfold Injective.
   intros.
   apply Hf with (C := Nil nat) (x := x) (y := y) (i := I) (j := I) in H.
@@ -46,9 +46,9 @@ Qed.
 
 (** reverse *)
 Proposition reverse_preserves_injectivity :
-  forall l T n, preserve_Injectivity reverse (l := l) (A := (n::T)).
+  forall T n, preserve_Injectivity reverse (A := (n::T)).
 Proof.
-  intros l T n C v Hinj i j x y H.
+  intros T n C v Hinj i j x y H.
   assert (function_injective : (forall (x y : Idx n), n - 1 - to_nat x = n - 1 - to_nat y -> x = y)). {
     intros x' y' H'. simpl in H'.
     apply sub_injective in H'.
@@ -88,9 +88,9 @@ Qed.
 
 (** take_left *)
 Proposition take_left_preserves_injectivity :
-  forall l T n b, preserve_Injectivity (take_left b) (l := l) (A := ((b+n)::T)).
+  forall T n b, preserve_Injectivity (take_left b) (A := ((b+n)::T)).
 Proof.
-  intros l T n b C v Hinj i j x y H.
+  intros T n b C v Hinj i j x y H.
   assert (function_injective : (forall (x y : Idx (b)), to_nat x = to_nat y -> x = y)). {
     intros x' y' H'.
     apply to_nat_injective in H'.
@@ -127,9 +127,9 @@ Qed.
 
 (** take_right *)
 Proposition take_right_preserves_injectivity :
-  forall l T n a, preserve_Injectivity (take_right a) (l := l) (A := ((a+n)::T)).
+  forall T n a, preserve_Injectivity (take_right a) (A := ((a+n)::T)).
 Proof.
-  intros l T n a C v Hinj i j x y H.
+  intros T n a C v Hinj i j x y H.
   assert (function_injective : (forall (x y : Idx n), a + to_nat x = a + to_nat y -> x = y)). {
     intros x' y' H'.
     apply add_injective in H'.
@@ -167,10 +167,10 @@ Qed.
 
 (** transpose *)
 Proposition transpose_preserves_injectivity :
-  forall l T m n, preserve_Injectivity transpose (l := l) (A := (m::n::T)).
+  forall T m n, preserve_Injectivity transpose (A := (m::n::T)).
 Proof.
   unfold preserve_Injectivity.
-  intros l T m n C v Hinj i j x y H.
+  intros T m n C v Hinj i j x y H.
   assert (function_injective : forall (i1 i2 : Idx m) (j1 j2: Idx n), (j1,i1) = (j2,i2) -> (i1,j1) = (i2,j2)). intros; inversion H0; subst; reflexivity.
   set (function := fun (x : Tuple (n::m::T)) => match x with | (i,(j,tx)) => (j,(i,tx)) end).
   simpl in H.
@@ -204,10 +204,10 @@ Qed.
 
 (** group *)
 Proposition group_preserves_injectivity :
-  forall l T m n, preserve_Injectivity (group m) (l := l) (A := (m*n::T)).
+  forall T m n, preserve_Injectivity (group m) (A := (m*n::T)).
 Proof.
   unfold preserve_Injectivity.
-  intros l T m n C v Hinj i j x y H.
+  intros T m n C v Hinj i j x y H.
   assert (function_injective : forall (xi yi : Idx n) (xj yj : Idx m), to_nat xj + m * to_nat xi = to_nat yj + m * to_nat yi -> (xi,xj) = (yi,yj)). {
     intros. apply projection_injective in H0.
     inversion H0. apply to_nat_injective in H2,H3. subst;reflexivity.
@@ -248,10 +248,10 @@ Qed.
 
 (** map *)
 Proposition map_preserves_injectivity :
-  forall l A B (n : nat) (f : ViewArray l A -> ViewArray l B), preserve_Injectivity f -> preserve_Injectivity (map f (n := n)).
+  forall A B (n : nat) (f : ViewArray A -> ViewArray B), preserve_Injectivity f -> preserve_Injectivity (map f (n := n)).
 Proof.
   unfold preserve_Injectivity.
-  intros l A B n f Hf C v Hinj i j x y H.
+  intros A B n f Hf C v Hinj i j x y H.
   assert (function_injective : forall (xi yi : Idx n) (tx ty : (Tuple B)),
       curry_totalApp (f (curry_partialApp v i xi)) tx = curry_totalApp (f (curry_partialApp v j yi)) ty ->
       ((xi,i),tx) = ((yi,j),ty)). {
